src/Common.v
@@ -29,6 +29,7 @@ Class set(T E: Type) := mkSet {
   singleton_set: E -> T;
   union: T -> T -> T;
   intersect: T -> T -> T;
+  diff: T -> T -> T;
   contains: T -> E -> Prop;
 }.
 
@@ -39,6 +40,7 @@ Instance Function_Set(E: Type): set (E -> Prop) E := {|
   singleton_set y := fun x => x = y;
   union := fun s1 s2 => fun x => s1 x \/ s2 x;
   intersect := fun s1 s2 => fun x => s1 x /\ s2 x;
+  diff := fun s1 s2 => fun x => s1 x /\ ~ s2 x;
   contains := id
 |}.
 
